Starting to port the H verification

opentheory/examples/all.ml
@@ -81,7 +81,9 @@ loads "opentheory/examples/char.ml";;
 (* Memory safety for the H interface.                                        *)
 (* ------------------------------------------------------------------------- *)
 
+(***
 loads "opentheory/examples/h.ml";;
+***)
 
 (* ------------------------------------------------------------------------- *)
 (* Map reduce example using Minisat.                                         *)
