opentheory/examples/stream.ml
@@ -18,6 +18,8 @@ let (snth_stream,stream_snth) =
 export_thm snth_stream;;
 export_thm stream_snth;;
 
+let stream_tybij = CONJ snth_stream stream_snth;;
+
 let shd_def = new_definition
   `!s : A stream. shd s = snth s 0`;;
 
@@ -47,6 +49,13 @@ let ssplit_def = new_definition
 
 export_thm ssplit_def;;
 
+let sinterleave_def = new_definition
+  `!s1 s2 : A stream.
+     sinterleave s1 s2 =
+     stream (\n. if EVEN n then snth s1 (n DIV 2) else snth s2 (n DIV 2))`;;
+
+export_thm sinterleave_def;;
+
 let sappend_def = new_definition
   `!l (s : A stream).
      sappend l s =
@@ -66,6 +75,24 @@ let snth_eq_imp = prove
    ASM_REWRITE_TAC [FUN_EQ_THM]);;
 
 export_thm snth_eq_imp;;
+
+let shd_scons = prove
+  (`!(h : A) t. shd (scons h t) = h`,
+   REPEAT STRIP_TAC THEN
+   REWRITE_TAC [shd_def; scons_def; stream_snth]);;
+
+export_thm shd_scons;;
+
+let stl_scons = prove
+  (`!(h : A) t. stl (scons h t) = t`,
+   REPEAT STRIP_TAC THEN
+   MATCH_MP_TAC snth_eq_imp THEN
+   GEN_TAC THEN
+   REWRITE_TAC
+     [stl_def; scons_def; sdrop_def; stream_snth; GSYM ADD1;
+      NOT_SUC; SUC_SUB1]);;
+
+export_thm stl_scons;;
 
 let snth_sappend = prove
   (`!l (s : A stream) n.
@@ -116,5 +143,73 @@ let sappend_assoc = prove
    REWRITE_TAC [ADD_ASSOC; ADD_SUB2]);;
 
 export_thm sappend_assoc;;
+
+let nil_sappend = prove
+  (`!s : A stream. sappend [] s = s`,
+   GEN_TAC THEN
+   MATCH_MP_TAC snth_eq_imp THEN
+   GEN_TAC THEN
+   REWRITE_TAC [sappend_def; LENGTH; LT; SUB_0; stream_snth]);;
+
+export_thm nil_sappend;;
+
+let cons_sappend = prove
+  (`!h t (s : A stream). sappend (CONS h t) s = scons h (sappend t s)`,
+   REPEAT GEN_TAC THEN
+   MATCH_MP_TAC snth_eq_imp THEN
+   GEN_TAC THEN
+   REWRITE_TAC [sappend_def; stream_snth; scons_def; LENGTH] THEN
+   NUM_CASES_TAC `n : num` THENL
+   [DISCH_THEN SUBST1_TAC THEN
+    REWRITE_TAC [LT_NZ; NOT_SUC; nth_0];
+    ALL_TAC] THEN
+   DISCH_THEN (X_CHOOSE_THEN `m : num` SUBST1_TAC) THEN
+   REWRITE_TAC [NOT_SUC; LT_SUC; SUC_SUB1] THEN
+   COND_CASES_TAC THENL
+   [REWRITE_TAC [] THEN
+    MATCH_MP_TAC nth_suc THEN
+    FIRST_ASSUM ACCEPT_TAC;
+    REWRITE_TAC [] THEN
+    AP_TERM_TAC THEN
+    POP_ASSUM (MP_TAC o REWRITE_RULE [NOT_LT; LE_EXISTS]) THEN
+    DISCH_THEN (CHOOSE_THEN SUBST1_TAC) THEN
+    REWRITE_TAC [GSYM SUC_ADD; ADD_SUB2]]);;
+
+export_thm cons_sappend;;
+
+let ssplit_sinterleave = prove
+  (`!s1 s2 : A stream. ssplit (sinterleave s1 s2) = (s1,s2)`,
+   REPEAT STRIP_TAC THEN
+   REWRITE_TAC [ssplit_def; sinterleave_def; PAIR_EQ] THEN
+   SUBGOAL_THEN `~(2 = 0)` ASSUME_TAC THENL
+   [NUM_REDUCE_TAC;
+    ALL_TAC] THEN
+   CONJ_TAC THENL
+   [MATCH_MP_TAC snth_eq_imp THEN
+    GEN_TAC THEN
+    REWRITE_TAC [stream_snth; EVEN_DOUBLE] THEN
+    AP_TERM_TAC THEN
+    MATCH_MP_TAC DIV_MULT THEN
+    FIRST_ASSUM ACCEPT_TAC;
+    MATCH_MP_TAC snth_eq_imp THEN
+    GEN_TAC THEN
+    REWRITE_TAC [stream_snth; GSYM NOT_ODD] THEN
+    SUBGOAL_THEN `ODD (2 * n + 1)`
+      (fun th ->
+         (SUBST1_TAC o EQT_INTRO) th THEN
+         (STRIP_ASSUME_TAC o REWRITE_RULE [ODD_MOD]) th) THENL
+    [REWRITE_TAC [GSYM ADD1; ODD_DOUBLE];
+     ALL_TAC] THEN
+    REWRITE_TAC [] THEN
+    AP_TERM_TAC THEN
+    MP_TAC (SPECL [`2`; `(2 * n + 1) DIV 2`; `n : num`] EQ_MULT_LCANCEL) THEN
+    ASM_REWRITE_TAC [] THEN
+    DISCH_THEN (SUBST1_TAC o SYM) THEN
+    MP_TAC (SPECL [`2 * n + 1 : num`; `2`] DIVISION_DEF_DIV) THEN
+    ASM_REWRITE_TAC [EQ_ADD_RCANCEL] THEN
+    DISCH_THEN (CONV_TAC o RAND_CONV o REWR_CONV o SYM) THEN
+    MATCH_ACCEPT_TAC MULT_SYM]);;
+
+export_thm ssplit_sinterleave;;
 
 logfile_end ();;
