opentheory/examples/probability.ml
@@ -5,18 +5,12 @@
 logfile "probability-def";;
 
 let (mk_dest_random,dest_mk_random) =
-  let exists = prove (`?(s : bool stream). T`, REWRITE_TAC []) in
-  let tybij =
-      REWRITE_RULE []
-        (new_type_definition "random" ("mk_random","dest_random") exists) in
-  let th1 = prove
-    (`!s. dest_random (mk_random s) = s`, REWRITE_TAC [tybij])
-  and th2 = prove
-    (`!r. mk_random (dest_random r) = r`, REWRITE_TAC [tybij]) in
-  (th1,th2);;
+  CONJ_PAIR (mk_newtype ("r","random") ("s",`:bool stream`));;
 
 export_thm mk_dest_random;;
 export_thm dest_mk_random;;
+
+let random_tybij = CONJ mk_dest_random dest_mk_random;;
 
 let rbit_def = new_definition
   `!r. rbit r = (shd (dest_random r), mk_random (stl (dest_random r)))`;;
